coq/NNRSimp/Lang/NNRSimpUsage.v
@@ -44,32 +44,6 @@ Section NNRSimpUsage.
        | NNRSimpGroupBy g sl e => nnrs_imp_expr_may_use e x
        end.
 
-  Lemma nnrs_imp_expr_may_use_free_vars e x :
-    nnrs_imp_expr_may_use e x = true <-> In x (nnrs_imp_expr_free_vars e).
-  Proof.
-    induction e; simpl; intuition; unfold equiv_decb in *.
-    - match_destr_in H; rewrite e; tauto.
-    - match_destr; congruence.
-    - rewrite in_app_iff.
-      apply orb_prop in H3.
-      tauto.
-    - rewrite in_app_iff in H3.
-      intuition.
-  Qed.
-
-  Lemma nnrs_imp_expr_may_use_free_vars_neg e x :
-    nnrs_imp_expr_may_use e x = false <-> ~ In x (nnrs_imp_expr_free_vars e).
-  Proof.
-    split; intros HH.
-    - intros H.
-      apply nnrs_imp_expr_may_use_free_vars in H.
-      congruence.
-    - case_eq (nnrs_imp_expr_may_use e x); trivial.
-      intros H.
-      apply nnrs_imp_expr_may_use_free_vars in H.
-      congruence.
-  Qed.
-  
   Inductive VarUsage :=
   | VarMustBeAssigned
   | VarMayBeUsedWithoutAssignment
@@ -138,4 +112,250 @@ Section NNRSimpUsage.
               end
        end.
 
+  Section vars.
+
+    Lemma nnrs_imp_expr_may_use_free_vars e x :
+      nnrs_imp_expr_may_use e x = true <-> In x (nnrs_imp_expr_free_vars e).
+    Proof.
+      induction e; simpl; intuition; unfold equiv_decb in *.
+      - match_destr_in H; rewrite e; tauto.
+      - match_destr; congruence.
+      - rewrite in_app_iff.
+        apply orb_prop in H3.
+        tauto.
+      - rewrite in_app_iff in H3.
+        intuition.
+    Qed.
+
+    Lemma nnrs_imp_expr_may_use_free_vars_neg e x :
+      nnrs_imp_expr_may_use e x = false <-> ~ In x (nnrs_imp_expr_free_vars e).
+    Proof.
+      split; intros HH.
+      - intros H.
+        apply nnrs_imp_expr_may_use_free_vars in H.
+        congruence.
+      - case_eq (nnrs_imp_expr_may_use e x); trivial.
+        intros H.
+        apply nnrs_imp_expr_may_use_free_vars in H.
+        congruence.
+    Qed.
+    
+    Lemma nnrs_imp_stmt_free_used s x :
+      nnrs_imp_stmt_var_usage s x <> VarNotUsedAndNotAssigned ->
+      In x (nnrs_imp_stmt_free_vars s).
+    Proof.
+      nnrs_imp_stmt_cases (induction s) Case
+      ; simpl
+      ; repeat rewrite in_app_iff
+      ; try rewrite nnrs_imp_expr_may_use_free_vars
+      ; try rewrite IHs
+      ; try rewrite IHs1
+      ; try rewrite IHs2.
+      - Case "NNRSimpSkip"%string.
+        congruence.
+      - Case "NNRSimpSeq"%string.
+        match_case; intuition congruence.
+      - Case "NNRSimpAssign"%string.
+        match_case; try congruence
+        ; try rewrite nnrs_imp_expr_may_use_free_vars
+        ; try rewrite nnrs_imp_expr_may_use_free_vars_neg.
+        + intuition congruence.
+        + unfold equiv_decb; destruct (v == x); intuition congruence.
+      - Case "NNRSimpLet"%string.
+        destruct o.
+        + (match_case; intros eqq)
+          ; try rewrite nnrs_imp_expr_may_use_free_vars in eqq
+          ; try rewrite nnrs_imp_expr_may_use_free_vars_neg in eqq.
+          * intuition congruence.
+          * { unfold equiv_decb; destruct (v == x); unfold equiv, complement in *.
+              - subst.
+                intuition.
+              - intuition.
+                right; apply remove_in_neq; intuition.
+            }
+        + simpl; intuition.
+          unfold equiv_decb in *; destruct (v ==x); try intuition congruence.
+          right.
+          apply remove_in_neq; intuition.
+      - Case "NNRSimpFor"%string.
+        (match_case; intros eqq)
+        ; try rewrite nnrs_imp_expr_may_use_free_vars in eqq
+        ; try rewrite nnrs_imp_expr_may_use_free_vars_neg in eqq.
+        + intuition congruence.
+        +  unfold equiv_decb; destruct (v == x); unfold equiv, complement in *.
+           * subst.
+             intuition.
+           * { match_case; intros eqq2; try congruence.
+               rewrite <- remove_in_neq by eauto.
+               right; apply IHs.
+               intuition; try congruence.
+             }
+      - Case "NNRSimpIf"%string.
+        (match_case; intros eqq)
+        ; try rewrite nnrs_imp_expr_may_use_free_vars in eqq
+        ; try rewrite nnrs_imp_expr_may_use_free_vars_neg in eqq.
+        + intuition congruence.
+        + match_case; intros eqq1
+          ; try (match_case; intros eqq2)
+          ; try intuition congruence.
+      - Case "NNRSimpEither"%string.
+        (match_case; intros eqq)
+        ; try rewrite nnrs_imp_expr_may_use_free_vars in eqq
+        ; try rewrite nnrs_imp_expr_may_use_free_vars_neg in eqq.
+        + intuition congruence.
+        + destruct (v == x).
+          * { destruct (v0 == x)
+              ; try intuition congruence.
+              match_case; intros eqq1
+              ; try (match_case; intros eqq2)
+              ; try intuition congruence.
+              right; right.
+              rewrite <- remove_in_neq by eauto.
+              apply IHs2; congruence.
+            } 
+          * { match_case; intros eqq1.
+              -  destruct (v0 == x)
+                 ; try intuition congruence.
+                 match_case; intros eqq2
+                 ; try intuition congruence.
+                 + right; left.
+                   rewrite <- remove_in_neq by eauto.
+                   apply IHs1; congruence.
+                 + right; left.
+                   rewrite <- remove_in_neq by eauto.
+                   apply IHs1; congruence.
+              -  right; left.
+                 rewrite <- remove_in_neq by eauto.
+                 apply IHs1; congruence.
+              - destruct (v0 == x)
+                ; try intuition congruence.
+                match_case; intros eqq2
+                ; try intuition congruence.
+                + right; right.
+                  rewrite <- remove_in_neq by eauto.
+                  apply IHs2; congruence.
+            }
+    Qed.
+
+    Lemma nnrs_imp_stmt_free_unassigned s x :
+      ~ In x (nnrs_imp_stmt_free_vars s) ->
+      nnrs_imp_stmt_var_usage s x = VarNotUsedAndNotAssigned.
+    Proof.
+      generalize (nnrs_imp_stmt_free_used s x); intros.
+      destruct (nnrs_imp_stmt_var_usage s x)
+      ; intuition congruence.
+    Qed.
+    
+  End vars.
+
+  Section eval.
+    
+    Lemma nnrs_imp_stmt_eval_must_assign_assigns {h σc s σ σ'}:
+      nnrs_imp_stmt_eval h σc s σ = Some σ' ->
+      forall x,
+        nnrs_imp_stmt_var_usage s x = VarMustBeAssigned ->
+        exists o, lookup equiv_dec σ' x = Some (Some o).
+    Proof.
+      intros eqq1 x; revert eqq1.
+      revert σ σ'.
+      nnrs_imp_stmt_cases (induction s) Case; simpl; intros σ σ' eq1 eq2.
+      - Case "NNRSimpSkip"%string.
+        congruence.
+      - Case "NNRSimpSeq"%string.
+        apply some_olift in eq1.
+        destruct eq1 as [? eqq1 eqq2].
+        symmetry in eqq2.
+        specialize (IHs1 _ _ eqq1).
+        specialize (IHs2 _ _ eqq2).
+        match_destr_in eq2; eauto.
+        destruct IHs1 as [o inn]; trivial.
+        generalize (nnrs_imp_stmt_eval_lookup_some_some eqq2 _ _ inn); trivial.
+      - match_destr_in eq2.
+        unfold equiv_decb in *.
+        destruct (v == x); try congruence.
+        match_destr_in eq1.
+        unfold equiv in *; subst.
+        match_option_in eq1.
+        invcs eq1.
+        apply lookup_in_domain in eqq.
+        rewrite lookup_update_eq_in; eauto.
+      - Case "NNRSimpLet"%string.
+        destruct o.
+        + match_destr_in eq2.
+          unfold equiv_decb in *.
+          destruct (v == x); try congruence.
+          unfold olift in eq1.
+          match_destr_in eq1.
+          match_option_in eq1.
+          destruct p; try discriminate.
+          invcs eq1.
+          specialize (IHs _ _ eqq eq2).
+          simpl in IHs.
+          destruct p.
+          apply nnrs_imp_stmt_eval_domain_stack in eqq.
+          simpl in eqq; invcs eqq.
+          match_destr_in IHs; try congruence.
+        + match_option_in eq1.
+          unfold equiv_decb in *.
+          destruct (v == x); try congruence.
+          destruct p; try discriminate.
+          invcs eq1.
+          specialize (IHs _ _ eqq eq2).
+          simpl in IHs.
+          destruct p.
+          apply nnrs_imp_stmt_eval_domain_stack in eqq.
+          simpl in eqq; invcs eqq.
+          match_destr_in IHs; try congruence.
+      - Case "NNRSimpFor"%string.
+        match_destr_in eq2.
+        unfold equiv_decb in *.
+        destruct (v == x); try congruence.
+        match_case_in eq2; intros eqq; rewrite eqq in *; try discriminate.
+      - Case "NNRSimpIf"%string.
+        match_destr_in eq1.
+        match_destr_in eq2.
+        match_case_in eq2; intros eqq1; rewrite eqq1 in *
+        ; try discriminate
+        ; match_case_in eq2; intros eqq2; rewrite eqq2 in *
+        ; try discriminate.
+
+        destruct d; try discriminate.
+        destruct b; eauto.
+      - Case "NNRSimpEither"%string.
+        match_destr_in eq1.
+        match_destr_in eq2.
+        destruct (v == x)
+        ; destruct (v0 == x)
+        ; try discriminate
+        ; try solve [repeat match_destr_in eq2; try congruence].
+        
+        match_case_in eq2; intros eqq1; rewrite eqq1 in *
+        ; try discriminate
+        ; match_case_in eq2; intros eqq2; rewrite eqq2 in *
+        ; try discriminate.
+
+        unfold var in *.
+        destruct d; try discriminate.
+        + match_option_in eq1.
+          destruct p; try discriminate.
+          specialize (IHs1 _ _ eqq eq2).
+          simpl in IHs1.
+          destruct p.
+          apply nnrs_imp_stmt_eval_domain_stack in eqq.
+          simpl in eqq; invcs eqq.
+          invcs eq1.
+          destruct (equiv_dec x s); try congruence.
+        + match_option_in eq1.
+          destruct p; try discriminate.
+          specialize (IHs2 _ _ eqq eq2).
+          simpl in IHs2.
+          destruct p.
+          apply nnrs_imp_stmt_eval_domain_stack in eqq.
+          simpl in eqq; invcs eqq.
+          invcs eq1.
+          destruct (equiv_dec x s); try congruence.
+    Qed.
+
+  End eval.
+  
 End NNRSimpUsage.
