coq/NNRSimp/Optim/TNNRSimpRewrite.v
@@ -20,10 +20,11 @@ Require Import String.
 Require Import List.
 Require Import ListSet.
 Require Import Arith.
-Require Import Equivalence.
 Require Import Morphisms.
 Require Import Setoid.
+Require Import Decidable.
 Require Import EquivDec.
+Require Import Equivalence.
 Require Import Program.
 Require Import Utils.
 Require Import CommonSystem.
@@ -54,6 +55,290 @@ Section TNNRSimpRewrite.
     apply nnrs_imp_stmt_eq_rewrites_to.
     - apply for_nil_eq.
     - eauto.
+  Qed.
+
+  Ltac disect_tac H stac
+    := 
+      unfold var in *
+      ; cut_to H; unfold domain in *; [ | solve[stac]..]
+      ; unfold lift2P in H
+      ; (repeat match_option_in H; try contradiction).
+
+  Ltac pcong
+    := solve[repeat (match goal with
+                     | [H: _ = _ |- _ ] => rewrite H in *; clear H
+                     end; try tauto)].
+
+  Ltac ren_eval_t stac
+    := repeat progress (
+                repeat rewrite in_app_iff in *
+                ; repeat
+                    match goal with
+                    | [H : ~ (_ \/ _ ) |- _ ] => apply not_or in H
+                    | [H : (_ \/ _ ) -> False |- _ ] => apply not_or in H
+                    | [H: _ /\ _ |- _ ] => destruct H
+                    | [ H : _ * _ |- _ ] => destruct H
+                    | [H: _::_ = _::_ |- _ ] => invcs H
+                    | [ H: domain (_ ++ _) = domain _ |- _ ] =>
+                      rewrite domain_app in H
+                      ; unfold domain in H
+                      ; symmetry in H; apply map_app_break in H
+                      ; destruct H as [? [?[?[??]]]]; subst; simpl in *
+                    | [ H: map (_ ++ _) = map _ |- _ ] =>
+                      rewrite map_app in H
+                      ; symmetry in H; apply map_app_break in H
+                      ; destruct H as [? [?[?[??]]]]; subst; simpl in *
+                    | [ H: _ :: _ = map _ ?x |- _ ] =>
+                      destruct x; try discriminate; simpl in H; invcs H
+                    | [ H: _ :: _ = domain ?x |- _ ] =>
+                      destruct x; try discriminate; simpl in H; invcs H
+                    | [H : ~ In _ (remove _ _ _) |- _ ] =>
+                      apply not_in_remove_impl_not_in in H; [| congruence]
+                    | [H : ?x ++ _ = ?y ++ _ |- _ ] =>
+                      let HH := fresh in
+                      assert (HH:domain y = domain x) by
+                          (unfold domain in *;
+                           try (intuition congruence)
+                           ; pcong)
+                      ; apply app_inv_head_domain in H;[clear HH|apply HH]
+                                                         
+
+                    | [ H: forall a b c, _ -> ?x1 ++ ?dd :: ?x2 = _ ++ _ :: _ -> _ |- _] =>
+                      specialize (H x1 (snd dd) x2); simpl in H
+                      ; match dd with
+                        | (_,_) => idtac
+                        | _ => destruct dd
+                        end
+                      ; simpl in *
+                      ; cut_to H; [ | eauto 3 | reflexivity]
+                    | [ H: forall a b c, _ -> ?dd0::?x1 ++ ?dd :: ?x2 = _ ++ _ :: _ -> _ |- _] =>
+                      specialize (H (dd0::x1) (snd dd) x2); simpl in H
+                      ; match dd with
+                        | (_,_) => idtac
+                        | _ => destruct dd
+                        end
+                      ; simpl in *
+                      ; cut_to H; [ | eauto 3 | reflexivity]
+                    | [ H: forall a b c, _ -> ?dd0::?dd :: ?x2 = _ ++ _ :: _ -> _ |- _] =>
+                      specialize (H (dd0::nil) (snd dd) x2); simpl in H
+                      ; match dd with
+                        | (_,_) => idtac
+                        | _ => destruct dd
+                        end
+                      ; simpl in *
+                      ; cut_to H; [ | eauto 3 | reflexivity]
+
+                    end
+                ; simpl in *; trivial; intros; try subst; try solve [congruence | f_equal; congruence]).          
+
+  Ltac ren_eval_tt := ren_eval_t ltac:(try tauto; try congruence).
+
+  Lemma let_let_coalesce_trew x₁ x₂ x₃ oe s₁ s₂ :
+    x₁ <> x₂ ->
+    ~ In x₁ (nnrs_imp_stmt_free_vars s₁) ->
+    ~ In x₃ (nnrs_imp_stmt_free_vars s₁) ->
+    ~ In x₃ (nnrs_imp_stmt_bound_vars s₁) ->
+    x₁ = x₃ \/ (~ In x₃ (nnrs_imp_stmt_free_vars s₂)
+                /\ ~ In x₃ (nnrs_imp_stmt_bound_vars s₂)) ->
+    NNRSimpLet x₁ None
+               (NNRSimpSeq
+                  (NNRSimpLet x₂ oe
+                              (NNRSimpSeq s₁
+                                          (NNRSimpAssign x₁ (NNRSimpVar x₂))))
+                  s₂)
+               ⇒ˢ
+               NNRSimpLet x₃
+               oe
+               (NNRSimpSeq (nnrs_imp_stmt_rename s₁ x₂ x₃)
+                           (nnrs_imp_stmt_rename s₂ x₁ x₃)).
+  Proof.
+    red; intros.
+    invcs H4.
+    invcs H9.
+    simpl in *.
+    invcs H7.
+    - case_eq (nnrs_imp_expr_may_use e₁ x₁)
+      ; intros nin1 ; rewrite nin1 in *; try congruence.
+      apply nnrs_imp_expr_may_use_free_vars_neg in nin1.
+      unfold equiv_decb in H8.
+      destruct (x₂ == x₁); try congruence.
+      destruct (x₁ == x₂); try congruence.
+      destruct (x₁ == x₁); try congruence.
+      assert (used1:nnrs_imp_stmt_var_usage s₁ x₁ <> VarMayBeUsedWithoutAssignment).
+      { destruct (nnrs_imp_stmt_var_usage s₁ x₁); congruence. }
+      clear H8.
+      invcs H12.
+      invcs H8.
+      invcs H11.
+      simpl in *.
+      destruct (string_dec x₁ x₂); try congruence.
+      destruct (string_dec x₁ x₁); try congruence.
+      unfold var in *.
+      destruct (equiv_dec x₂ x₂); try congruence.
+      invcs H12; invcs H6.
+      split.
+      + econstructor.
+        * eapply (nnrs_imp_expr_type_unused_remove _ nil) in H9
+          ; simpl; try tauto; eauto.
+        * { econstructor.
+            - apply nnrs_imp_stmt_type_rename_f; eauto.
+              eapply (nnrs_imp_expr_type_unused_remove _ nil) in H9
+              ; simpl; try tauto; eauto.
+              eapply (nnrs_imp_stmt_type_unused_remove Γc ((x₂, τ1)::nil)) in H7
+              ; simpl; eauto.
+            - destruct H3.
+              + subst.
+                rewrite nnrs_imp_stmt_rename_id; trivial.
+              + apply nnrs_imp_stmt_type_rename_f; eauto.
+                eapply (nnrs_imp_expr_type_unused_remove _ nil) in H9
+                ; simpl; try tauto; eauto.
+                eapply (nnrs_imp_stmt_type_unused_remove Γc ((x₂, τ1)::nil)) in H7
+                ; simpl; eauto; tauto.
+          }
+      + { intros.
+          generalize (nnrs_imp_expr_eval_unused brand_relation_brands σc nil); simpl
+          ; intros HH; rewrite HH; clear HH; try tauto.
+          case_eq ( (nnrs_imp_expr_eval brand_relation_brands σc σ e₁)); simpl; trivial.
+          intros ? eqq.
+          generalize (nnrs_imp_stmt_eval_unused brand_relation_brands σc ((x₂, Some d) :: nil) σ s₁ x₁ None); simpl; intros HH1.
+          cut_to HH1; [ | tauto].
+          generalize (nnrs_imp_stmt_eval_rename brand_relation_brands σc σ s₁ x₂ x₃ (Some d))
+          ; simpl; intros HH2.
+          cut_to HH2; [| tauto..].
+          unfold var in *.
+          unfold lift2P in HH1.
+          repeat match_option_in HH1
+          ; rewrite eqq1 in HH2
+          ; repeat match_option_in HH2
+          ; try contradiction
+          ; simpl
+          ; repeat (match_destr_in HH2; try contradiction).
+          generalize (nnrs_imp_stmt_eval_domain_stack eqq0)
+          ; generalize (nnrs_imp_stmt_eval_domain_stack eqq1)
+          ; generalize (nnrs_imp_stmt_eval_domain_stack eqq2)
+          ; intros.
+          ren_eval_tt.
+          destruct (s == s); try congruence.
+          destruct (string_dec s0 s); try congruence.
+          destruct (string_dec s0 s0); try congruence.
+          unfold id; simpl.
+          generalize (nnrs_imp_stmt_eval_preserves_some eqq1)
+          ; simpl; intros HH.
+          invcs HH.
+          cut_to H15; try congruence.
+          destruct o; simpl; try congruence.
+          destruct H3.
+          + subst.
+            rewrite nnrs_imp_stmt_rename_id; trivial.
+          + generalize (nnrs_imp_stmt_eval_rename brand_relation_brands σc p0 s₂ s0 x₃ (Some d0))
+            ; simpl; intros HH.
+            cut_to HH; [ | tauto..].
+            unfold var in *.
+            repeat match_option_in HH
+            ; (repeat match_destr_in HH; try contradiction).
+            intuition congruence.
+        }
+    - { simpl in H9.
+        unfold equiv_decb in *.
+        destruct (x₂ == x₂); try congruence.
+        match_case_in H9
+        ; intros eqq; rewrite eqq in *; try congruence.
+        invcs H12.
+        invcs H11.
+        invcs H12.
+        simpl in *.
+        destruct (string_dec x₁ x₂); try congruence.
+        destruct (string_dec x₁ x₁); try congruence.
+        unfold var in *.
+        destruct (equiv_dec x₂ x₂); try congruence.
+        invcs H13; invcs H6.
+        destruct (equiv_dec x₂ x₁); try congruence.
+        destruct (x₁ == x₁); try congruence.
+        destruct (x₁ == x₂); try congruence.
+        assert (used1:nnrs_imp_stmt_var_usage s₁ x₁ <> VarMayBeUsedWithoutAssignment).
+        { destruct (nnrs_imp_stmt_var_usage s₁ x₁); congruence. }
+        clear H8 c c0 e e0 e1 e2 n H9.
+        split.
+        - econstructor.
+          + simpl.
+            destruct (string_dec x₂ x₃).
+            * subst.
+              rewrite nnrs_imp_stmt_rename_id, eqq; congruence.
+            * rewrite nnrs_imp_stmt_rename_var_usage_eq_to by trivial.
+              rewrite eqq.
+              congruence.
+          + { econstructor.
+              - apply nnrs_imp_stmt_type_rename_f; eauto.
+                eapply (nnrs_imp_stmt_type_unused_remove Γc ((x₂, τ1)::nil)) in H7
+                ; simpl; eauto.
+              - destruct H3.
+                + subst.
+                  rewrite nnrs_imp_stmt_rename_id; trivial.
+                + apply nnrs_imp_stmt_type_rename_f; eauto; try tauto.
+            }        
+        - intros.
+          generalize (nnrs_imp_stmt_eval_unused brand_relation_brands σc ((x₂, None) :: nil) σ s₁ x₁ None); simpl; intros HH1.
+          cut_to HH1; [ | tauto].
+          generalize (nnrs_imp_stmt_eval_rename brand_relation_brands σc σ s₁ x₂ x₃ None)
+          ; simpl; intros HH2.
+          cut_to HH2; [| tauto..].
+          unfold var in *.
+          unfold lift2P in HH1.
+          repeat match_option_in HH1
+          ; rewrite eqq1 in HH2
+          ; repeat match_option_in HH2
+          ; try contradiction
+          ; simpl
+          ; repeat (match_destr_in HH2; try contradiction).
+          generalize (nnrs_imp_stmt_eval_domain_stack eqq0)
+          ; generalize (nnrs_imp_stmt_eval_domain_stack eqq1)
+          ; generalize (nnrs_imp_stmt_eval_domain_stack eqq2)
+          ; intros.
+          destruct HH2 as [?[?[??]]]; subst.
+          ren_eval_tt.
+          destruct (s == s); try congruence.
+          destruct (string_dec s0 s); try congruence.
+          destruct (string_dec s0 s0); try congruence.
+          unfold id; simpl.
+          destruct (nnrs_imp_stmt_eval_must_assign_assigns eqq1 s eqq)
+            as [dd ddin].
+          simpl in ddin.
+          match_destr_in ddin; try congruence.
+          invcs ddin.
+          simpl.
+          destruct H3.
+          + subst.
+            rewrite nnrs_imp_stmt_rename_id; trivial.
+          + generalize (nnrs_imp_stmt_eval_rename brand_relation_brands σc p0 s₂ s0 x₃ (Some dd))
+            ; simpl; intros HH.
+            cut_to HH; [ | tauto..].
+            unfold var in *.
+            repeat match_option_in HH
+            ; (repeat match_destr_in HH; try contradiction).
+            intuition congruence.
+      } 
+  Qed.
+  
+  Lemma let_let_coalesce_trew1 x₁ x₂ oe s₁ s₂ :
+    x₁ <> x₂ ->
+    ~ In x₁ (nnrs_imp_stmt_free_vars s₁) ->
+    ~ In x₁ (nnrs_imp_stmt_bound_vars s₁) ->
+    NNRSimpLet x₁ None
+               (NNRSimpSeq
+                  (NNRSimpLet x₂ oe
+                              (NNRSimpSeq s₁
+                                          (NNRSimpAssign x₁ (NNRSimpVar x₂))))
+                  s₂)
+               ⇒ˢ
+               NNRSimpLet x₁ oe
+               (NNRSimpSeq (nnrs_imp_stmt_rename s₁ x₂ x₁)
+                           s₂).
+  Proof.
+    intros.
+    generalize (let_let_coalesce_trew x₁ x₂ x₁ oe s₁ s₂)
+    ; simpl; intros HH.
+    rewrite nnrs_imp_stmt_rename_id in HH.
+    apply HH; try tauto.
   Qed.
 
 End TNNRSimpRewrite.
